rewrite the invs

impl/riscv/mod32_lemmas.i.dfy
@@ -16,77 +16,74 @@ module mod32_lemmas {
   const B2 : int := B * B;
 
   predicate sub_mod32_loop_inv(
-    iter_a: iter_t,
-    iter_n: iter_t,
-    iter_a': iter_t,
+    old_a: seq<uint32>,
+    n: seq<uint32>,
+    a: seq<uint32>,
+    i: nat,
     A: int64_view_t)
   {
     && sub_mod32_A_inv(A)
-    && var i := iter_a.index;
-    && |iter_a.buff| == |iter_n.buff| == |iter_a'.buff|
-    && (i == iter_a'.index == iter_n.index)
-    && i <= |iter_a.buff|
-    && iter_a.buff[i..] == iter_a'.buff[i..]
-    && SeqSub(iter_a.buff[..i], iter_n.buff[..i]) == (iter_a'.buff[..i], A_as_carry(A.full))
+    && |old_a| == |a| == |n|
+    && 0 <= i <= |a|
+    && old_a[i..] == a[i..]
+    && SeqSub(old_a[..i], n[..i]) == (a[..i], A_as_carry(A.full))
   }
 
   lemma lemma_sub_mod32_correct(
     A: int64_view_t,
-    iter_a: iter_t, iter_n: iter_t, iter_a': iter_t,
-    iter_a_next: iter_t, iter_n_next: iter_t, iter_a'_next: iter_t,
+    old_a: seq<uint32>, n: seq<uint32>, a: seq<uint32>,
     v0: uint32, v1: uint32,
     lh: uint32, uh: uint32,
     carry_add: int, carry_sub: int,
     x13: uint32,
-    i: int)
+    i: nat)
   returns  (A': int64_view_t)
 
-  requires sub_mod32_loop_inv(iter_a, iter_n, iter_a', A)
-  requires iter_a.index < |iter_a.buff|
-  requires i == iter_a.index
+  requires sub_mod32_loop_inv(old_a, n, a, i, A)
+  requires i < |a|
 
-  requires v0 == uint32_add(A.lh, iter_a.buff[i]);
-  requires x13 == uint32_sub(v0, iter_n.buff[i]);
+  requires v0 == uint32_add(A.lh, old_a[i]);
+  requires x13 == uint32_sub(v0, n[i]);
 
-  requires carry_add == uint32_lt(v0, iter_a.buff[i]);
+  requires carry_add == uint32_lt(v0, old_a[i]);
   requires carry_sub == uint32_lt(v0, x13);
   requires v1 == uint32_add(A.uh, carry_add);
 
   requires lh == uint32_sub(v1, carry_sub);
   requires uh == to_uint32(int32_rs(to_int32(lh), 31));
 
-  requires iter_a_next == lw_next_iter(iter_a)
-  requires iter_n_next == lw_next_iter(iter_n)
-  requires iter_a'_next == sw_next_iter(iter_a', x13)
-
-  ensures sub_mod32_loop_inv(iter_a_next, iter_n_next, iter_a'_next, A')
   ensures A' == int64_cons(lh, uh, A'.full)
+  ensures sub_mod32_loop_inv(old_a, n, a[i := x13], i + 1, A')
   {
-    var a_i := iter_a_next.buff[i];
-    var n_i := iter_n_next.buff[i];
+    var a_i := old_a[i];
+    var n_i := n[i];
 
-    var (zs_next, bin_next) := SeqSub(iter_a_next.buff[..i+1], iter_n_next.buff[..i+1]);
-    var (zs, _) := SeqSub(iter_a.buff[..i], iter_n.buff[..i]);
-    
+    assert a_i == a[i];
+
+    var (zs_next, bin_next) := SeqSub(old_a[..i+1], n[..i+1]);
+    var (zs, _) := SeqSub(old_a[..i], n[..i]);
+
     A' := update_A_correct(A, a_i, n_i, v0, v1, lh, uh, carry_add, carry_sub);
-
     var (z, bout) := uint32_subb(a_i, n_i, A_as_carry(A.full));
 
     calc {
       zs_next;
       {
-        assert(iter_a_next.buff[..i+1][..i] == iter_a.buff[..i]);
-        assert(iter_n_next.buff[..i+1][..i] == iter_n.buff[..i]);
+        assert(old_a[..i+1][..i] == old_a[..i]);
+        assert(n[..i+1][..i] == n[..i]);
         reveal SeqSub();
       }
       zs + [x13];
-      iter_a'.buff[..i] + [x13];
-      iter_a'_next.buff[..i+1];
+      {
+        assert zs == a[..i];
+      }
+      a[..i] + [x13];
+      a[i := x13][..i+1];
     }
 
     assert bin_next == if a_i >= n_i + A_as_carry(A.full) then 0 else 1 by {
-      assert(iter_a_next.buff[..i+1][..i] == iter_a.buff[..i]);
-      assert(iter_n_next.buff[..i+1][..i] == iter_n.buff[..i]);
+      assert(old_a[..i+1][..i] == old_a[..i]);
+      assert(n[..i+1][..i] == n[..i]);
       reveal SeqSub();
     }
 
@@ -95,57 +92,56 @@ module mod32_lemmas {
     }
   }
 
-  lemma sub_mod32_post_lemma(iter_a: iter_t, iter_n: iter_t, iter_a': iter_t, A: int64_view_t)
-    requires sub_mod32_loop_inv(iter_a, iter_n, iter_a', A);
-    requires iter_a.index == |iter_a.buff|
-    ensures to_nat(iter_a'.buff) ==
-      to_nat(iter_a.buff) - to_nat(iter_n.buff) + A_as_carry(A.full) * Power.Pow(BASE_32, |iter_a.buff|)
+  lemma sub_mod32_post_lemma(old_a: seq<uint32>, n: seq<uint32>, a: seq<uint32>, A: int64_view_t)
+    requires sub_mod32_loop_inv(old_a, n, a, |a|, A);
+    ensures to_nat(a) ==
+      to_nat(old_a) - to_nat(n) + A_as_carry(A.full) * Power.Pow(BASE_32, |old_a|)
   {
-    var i := iter_a.index;
-    assert iter_a.buff[..i] == iter_a.buff;
-    assert iter_n.buff[..i] == iter_n.buff;
-    assert iter_a'.buff[..i] == iter_a'.buff;
+    var i := |old_a|;
+    assert old_a[..i] == old_a;
+    assert n[..i] == n;
+    assert a[..i] == a;
     var cout := A_as_carry(A.full);
-    assert SeqSub(iter_a.buff, iter_n.buff) == (iter_a'.buff, cout);
-    LemmaSeqSub(iter_a.buff, iter_n.buff, iter_a'.buff, cout);
+    assert SeqSub(old_a, n) == (a, cout);
+    LemmaSeqSub(old_a, n, a, cout);
   }
 
     // predicate ge_mod32_loop_inv(
-    //   iter_a: iter_t,
-    //   iter_n: iter_t,
+    //   old_a: iter_t,
+    //   n: iter_t,
     //   cond: uint1,
     //   b: bool)
     // {
-    //   var i := iter_a.index;
-    //   && cond != 0 ==> 0 <= i < |iter_a.buff|
-    //   && cond == 0 ==> -1 <= i < |iter_a.buff|- 1
-    //   && cond == 1 ==> iter_a.buff[i+1..] == iter_n.buff[i+1..]
-    //   && (cond == 0 ==> (b ==> iter_a.buff[i+1] > iter_n.buff[i+1]) || (iter_a.buff == iter_n.buff))
-    //   && cond == 0 ==> (ToNatRight(iter_a.buff) >= ToNatRight(iter_n.buff)) == b
+    //   var i := old_a.index;
+    //   && cond != 0 ==> 0 <= i < |old_a|
+    //   && cond == 0 ==> -1 <= i < |old_a|- 1
+    //   && cond == 1 ==> old_a[i+1..] == n[i+1..]
+    //   && (cond == 0 ==> (b ==> old_a[i+1] > n[i+1]) || (old_a == n))
+    //   && cond == 0 ==> (ToNatRight(old_a) >= ToNatRight(n)) == b
     // }
 
     // lemma lemma_ge_mod32_correct(
-    //   iter_a: iter_t,
-    //   iter_n: iter_t,
-    //   iter_a_prev: iter_t,
-    //   iter_n_prev: iter_t,
+    //   old_a: iter_t,
+    //   n: iter_t,
+    //   old_a_prev: iter_t,
+    //   n_prev: iter_t,
     //   cond: uint1,
     //   b: bool,
     //   i: int)
     //   requires
-    //     && ge_mod32_loop_inv(iter_a, iter_n, cond, b)
+    //     && ge_mod32_loop_inv(old_a, n, cond, b)
 
-    //     && iter_a.index < |iter_a.buff|
-    //     && i == iter_a.index == iter_n.index
+    //     && old_a.index < |old_a|
+    //     && i == old_a.index == n.index
     //     && i > 0
 
     //     //&& cond == uint32_lt(0, uint32_xor(x11, x15)) // cond = x12
-    //     && cond == iter_n.index == |iter_n.buff| - 1
+    //     && cond == n.index == |n| - 1
 
-    //     && iter_a_prev == lw_prev_iter(iter_a)
-    //     && iter_n_prev == lw_prev_iter(iter_n)
+    //     && old_a_prev == lw_prev_iter(old_a)
+    //     && n_prev == lw_prev_iter(n)
     //   ensures
-    //     ge_mod32_loop_inv(iter_a_prev, iter_n_prev, cond, b)
+    //     ge_mod32_loop_inv(old_a_prev, n_prev, cond, b)
     // {
     // }
 
